PropositionalLogic/DeepEmbeddedInstance/TrivialSemantics.v
@@ -1,0 +1,37 @@
+Require Import Coq.Logic.Classical_Prop.
+Require Import Logic.lib.Ensembles_ext.
+Require Import Logic.GeneralLogic.Base.
+Require Import Logic.MinimunLogic.Syntax.
+Require Import Logic.PropositionalLogic.Syntax.
+Require Import Logic.PropositionalLogic.Semantics.TrivialSemantics.
+Require Import Logic.PropositionalLogic.DeepEmbeddedInstance.PropositionalLanguage.
+
+Definition model (Var: Type): Type := Var -> Prop.
+
+Fixpoint denotation {Var: Type} (x: expr Var): Ensemble (model Var) :=
+  match x with
+  | andp y z => Semantics.andp (denotation y) (denotation z)
+  | orp y z => Semantics.orp (denotation y) (denotation z)
+  | impp y z => Semantics.impp (denotation y) (denotation z)
+  | falsep => Semantics.falsep
+  | varp p => fun m => m p
+  end.
+
+Instance MD (Var: Type): Model :=
+  Build_Model (model Var).
+
+Instance SM (Var: Type): Semantics (PropositionalLanguage.L Var) (MD Var)  :=
+  Build_Semantics (PropositionalLanguage.L Var) (MD Var) denotation.
+
+Instance tpSM (Var: Type): TrivialPropositionalSemantics (L Var) (MD Var) (SM Var).
+Proof.
+  constructor.
+  + simpl; intros.
+    apply Same_set_refl.
+  + simpl; intros.
+    apply Same_set_refl.
+  + simpl; intros.
+    apply Same_set_refl.
+  + simpl; intros.
+    apply Same_set_refl.
+Qed.
