PropositionalLogic/Semantics/Kripke.v
@@ -1,7 +1,8 @@
 Require Import Coq.Logic.Classical_Prop.
 Require Import Coq.Classes.RelationClasses.
 Require Import Coq.Relations.Relation_Definitions.
-Require Import Logic.MinimunLogic.LogicBase.
+Require Import Logic.GeneralLogic.Base.
+Require Import Logic.MinimunLogic.Syntax.
 Require Import Logic.PropositionalLogic.Syntax.
 
 Local Open Scope logic_base.
