PropositionalLogic/Semantics/Trivial.v
@@ -1,0 +1,62 @@
+Require Import Coq.Logic.Classical_Prop.
+Require Import Logic.GeneralLogic.Base.
+Require Import Logic.MinimunLogic.Syntax.
+Require Import Logic.PropositionalLogic.Syntax.
+
+Local Open Scope logic_base.
+Local Open Scope syntax.
+Import PropositionalLanguageNotation.
+
+Module Semantics.
+
+Definition impp {model: Type} (X: Ensemble model) (Y: Ensemble model): Ensemble model :=
+  fun m => X m -> Y m.
+
+Definition andp {model: Type} (X: Ensemble model) (Y: Ensemble model): Ensemble model :=
+  fun m => X m /\ Y m.
+
+Definition orp {model: Type} (X: Ensemble model) (Y: Ensemble model): Ensemble model :=
+  fun m => X m \/ Y m.
+
+Definition falsep {model: Type}: Ensemble model := fun m => False.
+
+End Semantics.
+
+Class TrivialPropositionalSemantics (L: Language) {nL: NormalLanguage L} {pL: PropositionalLanguage L} (MD: Model) (SM: Semantics L MD): Type := {
+  denote_andp: forall x y, Same_set _ (denotation (x && y)) (Semantics.andp (denotation x) (denotation y));
+  denote_orp: forall x y, Same_set _ (denotation (x || y)) (Semantics.orp (denotation x) (denotation y));
+  denote_impp: forall x y, Same_set _ (denotation (x --> y)) (Semantics.impp (denotation x) (denotation y));
+  denote_falsep: Same_set _ (denotation FF) Semantics.falsep
+}.
+
+Lemma sat_andp {L: Language} {nL: NormalLanguage L} {pL: PropositionalLanguage L} {MD: Model} {SM: Semantics L MD} {tpSM: TrivialPropositionalSemantics L MD SM}: forall m x y, m |= x && y <-> (m |= x /\ m |= y).
+Proof.
+  intros; simpl.
+  unfold satisfies.
+  destruct (denote_andp x y).
+  split; auto; [apply H | apply H0].
+Qed.
+
+Lemma sat_orp {L: Language} {nL: NormalLanguage L} {pL: PropositionalLanguage L} {MD: Model} {SM: Semantics L MD} {tpSM: TrivialPropositionalSemantics L MD SM}: forall m x y, m |= x || y <-> (m |= x \/ m |= y).
+Proof.
+  intros; simpl.
+  unfold satisfies.
+  destruct (denote_orp x y).
+  split; auto; [apply H | apply H0].
+Qed.
+
+Lemma sat_impp {L: Language} {nL: NormalLanguage L} {pL: PropositionalLanguage L} {MD: Model} {SM: Semantics L MD} {tpSM: TrivialPropositionalSemantics L MD SM}: forall m x y, m |= x --> y <-> (m |= x -> m |= y).
+Proof.
+  intros; simpl.
+  unfold satisfies.
+  destruct (denote_impp x y).
+  split; auto; [apply H | apply H0].
+Qed.
+
+Lemma sat_falsep {L: Language} {nL: NormalLanguage L} {pL: PropositionalLanguage L} {MD: Model} {SM: Semantics L MD} {tpSM: TrivialPropositionalSemantics L MD SM}: forall m, m |= FF <-> False.
+Proof.
+  intros; simpl.
+  unfold satisfies.
+  destruct denote_falsep.
+  split; auto; [apply H | apply H0].
+Qed.
